\begin{align*}
    s = \frac{x_s - x_0}{h} = \frac{1.4321 - 0}{ 0.3142 - 0} = 4.5579
\end{align*}

\begin{align*}
    f'(x) = \frac{d(f(x))}{dx} =~&~  \frac{1}{h} \Bigg[ \Delta f_{-1} + \frac{2s + 1}{2!} \Delta^2 f_{-2} + \frac{3s^2 + 6s + 2}{3!} \Delta^3 f_{-3} \\
        &~+ \frac{4s^3 + 18s^2 + 22s + 6}{4!} \Delta^4 f_{-4} \\
        &~+ \frac{5s^4 + 40s^3 + 105s^2 + 100s + 24}{5!} \Delta^5 f_{-5}
        \Bigg]
\end{align*}

\begin{align*}
    \frac{2s + 1}{2!} = \frac{2(4.5579) + 1}{2} = 5.0579
\end{align*}

\begin{align*}
    \frac{3s^2 + 6s + 2}{3!} = \frac{3(4.5579)^2 + 6(4.5579) + 2}{6} = 15.2785
\end{align*}

\begin{align*}
    \frac{4s^3 + 18s^2 + 22s + 6}{4!} = \frac{4(4.5579)^3 + 18(4.5579)^2 + 22(4.5579) + 6}{24} = 35.7902
\end{align*}

\begin{multline*}
    \frac{5s^4 + 40s^3 + 105s^2 + 100s + 24}{5!} \\
    = \frac{5(4.5579)^4 + 40(4.5579)^3 + 105(4.5579)^2 + 100(4.5579) + 24}{120} \\
    = 71.7209
\end{multline*}

\begin{align*}
    f'(x) = \frac{d(f(x))}{dx} =~&~  \frac{1}{h} \Bigg[ \Delta f_{-1} + \frac{2s + 1}{2!} \Delta^2 f_{-2} + \frac{3s^2 + 6s + 2}{3!} \Delta^3 f_{-3} \\
        &~+ \frac{4s^3 + 18s^2 + 22s + 6}{4!} \Delta^4 f_{-4} \\
        &~+ \frac{5s^4 + 40s^3 + 105s^2 + 100s + 24}{5!} \Delta^5 f_{-5}
        \Bigg] \\
        =~&~  \frac{1}{0.3142} \Bigg[ 0.9862 + (5.0579) (0.0112) + (15.2785) (-0.0278) \\
        &~+ (35.7902) (0.0155) + (71.7209) (0.0042)
        \Bigg] \\
        =~&~ 4.6915
\end{align*}

(1 / 0.3142) * (  0.9862 + (5.0579)*(0.0112) + (15.2785)*(-0.0278) + (35.7902)*(0.0155) + (71.7209)*(0.0042) )