\begin{align*}
    s &= \frac{x_s - x_0}{h} \\
    &= \frac{0.9748 - 0.7854}{1.1781 - 1.5708} \\
    &= \frac{0.18940}{-0.39270} \\
    &= -0.4823
\end{align*}

\begin{align*}
f(x_s) &= f_0 +
    \left| \begin{array}{c} s \\ 1 \end{array} \right|
    \frac{\Delta f_{-1} + \Delta f_0}{2}
    + \frac{
        \left| \begin{array}{c} s + 1 \\ 2 \end{array} \right|
        + \left| \begin{array}{c} s \\ 2 \end{array} \right|
        }{2} \Delta^2 f_{-1} \\
&+ \left| \begin{array}{c} s + 1 \\ 3 \end{array} \right|
    \frac{\Delta^3 f_{-2} + \Delta^3 f_{-1}}{2}
    + \frac{
        \left| \begin{array}{c} s + 2 \\ 4 \end{array} \right|
        + \left| \begin{array}{c} s + 1 \\ 4 \end{array} \right|
        }{2} \Delta^4 f_{-2}
\end{align*}

\begin{align*}
\left| \begin{array}{c} s \\ 1 \end{array} \right| &= s \\
        &= -0.4823
\end{align*}

\begin{align*}
\left| \begin{array}{c} s + 1 \\ 2 \end{array} \right| + \left| \begin{array}{c} s \\ 2 \end{array} \right| &= \frac{(s+1)(s)}{2 !} + \frac{(s)(s-1)}{2 !} \\
    &= \frac{(-0.4823+1)(-0.4823)}{2 !} + \frac{(-0.4823)(-0.4823-1)}{2 !} \\
    &= -0.12484 + 0.35746 \\
    &= 0.23262
\end{align*}

\begin{align*}
\left| \begin{array}{c} s + 1 \\ 3 \end{array} \right| &= \frac{(s+1)(s)(s-1)}{3!} \\
    &= \frac{(-0.4823 + 1)(-0.4823)(-0.4823 - 1)}{6} \\
    &= 0.061685
\end{align*}

\begin{align*}
\left| \begin{array}{c} s + 2 \\ 4 \end{array} \right| + \left| \begin{array}{c} s + 1 \\ 4 \end{array} \right| =&~ \frac{(s+2)(s+1)(s)(s-1)}{4!} + \frac{(s+1)(s)(s-1)(s-2)}{4!} \\
    =&~ \frac{(-0.4823+2)(-0.4823+1)(-0.4823)(-0.4823-1)}{24} \\
    &~+ \frac{(-0.4823+1)(-0.4823)(-0.4823-1)(-0.4823-2)}{24} \\
    =&~ 0.023405 + (-0.038280) \\
    =&~ -0.014875
\end{align*}

\begin{align*}
f(x_s) &=~ 0.7071 ~+~ (-0.4823) ~\frac{(-0.2168) ~+~ (-0.3244)}{2} \\
    &~+~ \frac{0.23262}{2} (-0.1076) ~+~ (0.061685) \frac{0.0330 ~+~ 0.0494}{2} \\
    &~+~ \frac{-0.014875}{2} 0.0164 \\
    &=~ 0.7071 ~+~ (0.13051) ~+~ (-0.012515) ~+~ (-0.00012198) \\
    &=~ 0.82497
\end{align*}